Rearranged file structure, defining the concurrent semantics for assembly

x86/AsmMulti.v
@@ -10,98 +10,38 @@ Require Import Smallstep.
 Require Import SmallstepClosed.
 Require Import Values Maps Memory AST.
 
-Module NatIndexed.
-    Definition t := nat.
+Require Import Asm SmallstepMulti.
 
-    Definition index (n : nat) : positive :=
-      match n with
-      |O => 1%positive
-      |_ => 1 + Pos.of_nat n
-      end.
-
-    Definition index_rev (p:positive) : nat :=
-      match p with
-      |xH => O
-      |_ => Pos.to_nat p -1
-    end.
-
-    Lemma t_positive_t : forall (n:nat), index_rev (index n) = n.
-    Proof.
-      intros.
-      destruct (index n) eqn:Hn; unfold index_rev; destruct n; unfold index in *; lia.
-    Qed.
-
-    Lemma positive_t_positive : forall (p:positive), index(index_rev p) = p.
-    Proof.
-      intros. destruct (index_rev p) eqn:Hp; unfold index; destruct p; unfold index_rev in *; lia.
-    Qed.
-
-    Lemma index_inj : forall (x y : nat), index x = index y -> x = y.
-    Proof.
-      destruct x; destruct y; unfold index in *; lia.
-    Qed.
-    
-    Definition eq := Nat.eq_dec.
-End NatIndexed.
-
-Module NatMap := IRMap(NatIndexed).
-
-(** Unchecked concern: Do we need to define new events for [yield] and [pthread_create] ? Can we keep the internal events?
-    Now this two points are implemented differernt with CASCompCert *)
 Section MultiThread.
-
-  Context {OpenS : semantics li_c li_c}.
-
-  Definition local_state := state OpenS.
-
-  Record cq_vals : Type := cqv {cqv_vf : val; cqv_sg : signature; cqv_args : list val}.
-
-  Definition get_query (cqv : cq_vals) (m: mem) :=
-    cq (cqv_vf cqv) (cqv_sg cqv) (cqv_args cqv) m.
-
-  Definition get_cqv (q: c_query) :=
-    cqv (cq_vf q) (cq_sg q) (cq_args q).
   
-  Definition thread_state :Type := local_state + cq_vals.
-  
-  (* Maybe should be somehow added into open semantics *)
-  Variable initial_query : query li_c.
-  Variable final_reply : int -> reply li_c -> Prop.
+  Context {OpenS: Smallstep.semantics li_asm li_asm}.
 
-  (* should be derived from skel of OpenS
-     and allocate blocks for pthread primitives *)
+  Definition local_state := Smallstep.state OpenS.
+
+  Definition thread_state : Type := local_state + regset.
+
+  Variable initial_query : query li_asm.
+  Variable final_reply : int -> reply li_asm -> Prop.
+
   Variable initial_se : Genv.symtbl.
-  
+
   Definition OpenLTS := activate OpenS initial_se.
   Definition ClosedS := Closed.close_semantics initial_query final_reply OpenS initial_se.
 
-  (* We need an interface to get and set global memory from local_state *)
-  (* Not sure if this is proper, maybe need some lemmas about these operations *)
-
-  (*Variable get_gmem : local_state -> mem.
-  Variable set_gmem : mem -> local_state -> local_state. *)
-  
-  (** * Definition and operations of global state *)
-
-    Record state : Type := mk_gstate
-    {
-      threads: NatMap.t (option thread_state);
-      cur_tid : nat;
-      next_tid : nat;
-      (* atom_bit : bool; *)
-
-      (* tid_gmem : exists ls, NatMap.get cur_tid threads = Some ls /\
-                         tid_mem (get_gmem ls) = cur_tid /\
-                         length (stacks_mem (get_gmem ls)) = next_tid; *)
-    }.
+  Record state : Type := mk_gstate_asm
+      {
+        threads : NatMap.t (option thread_state);
+        cur_tid : nat;
+        next_tid : nat;
+      }.
 
   Definition empty_threads : NatMap.t (option thread_state) := NatMap.init None.
   
   Definition update_threads (s: state) (t: NatMap.t (option thread_state)) :=
-    mk_gstate t (cur_tid s) (next_tid s) .
+    mk_gstate_asm t (cur_tid s) (next_tid s) .
 
   Definition update_thread (s: state) (tid : nat) (ls: thread_state) :=
-    mk_gstate (NatMap.set tid (Some ls) (threads s)) (cur_tid s) (next_tid s).
+    mk_gstate_asm (NatMap.set tid (Some ls) (threads s)) (cur_tid s) (next_tid s).
 
   Definition update_cur_thread (s: state) (ls : thread_state) := update_thread s (cur_tid s) ls.
   
@@ -111,17 +51,13 @@ Section MultiThread.
   Definition get_cur_thread (s: state) := get_thread s (cur_tid s).
   
   Definition update_cur_tid (s: state) (tid : nat) :=
-    mk_gstate (threads s) tid (next_tid s).
+    mk_gstate_asm (threads s) tid (next_tid s).
 
   Definition update_next_tid (s: state) (tid: nat) :=
-    mk_gstate (threads s) (cur_tid s) tid.
+    mk_gstate_asm (threads s) (cur_tid s) tid.
   
   Variable yield_strategy : state -> nat.
   Axiom yield_strategy_range : forall s, (1 < yield_strategy s < (next_tid s))%nat.
-  (*some other properties may be added here, such as only point to active threads *)
-
-  (* We transfer to thread tid' and update
-     its local_state with an updated memory *)
 
   Definition yield_state (s: state) (ls: thread_state): state :=
     let tid' := yield_strategy s in
@@ -130,19 +66,14 @@ Section MultiThread.
 
   (* We add a new thread with its initial query without memory,
       we also update the running memory by adding a new list of positives *)
-  Definition pthread_create_state (s: state) (cqv : cq_vals) (ls' : thread_state): state :=
+  Definition pthread_create_state (s: state) (regs: regset) (ls' : thread_state): state :=
     let ntid := (next_tid s) in let ctid := (cur_tid s) in
     let s' := update_next_tid s (S ntid) in
-    let s'' := update_thread s' ntid (inr cqv) in
+    let s'' := update_thread s' ntid (inr regs) in
     update_thread s'' ctid ls'.
     
   Definition genvtype := Smallstep.genvtype OpenLTS.
   
-  (** Initial state of Concurrent semantics *)
-
-  (* We need a "query" to the main function of the semantics *)
-  (* Including the initial global memory *)
-
   Inductive initial_state : state -> Prop :=
   |initial_state_intro : forall ls s,
       cur_tid s = 1%nat -> next_tid s = 2%nat ->
@@ -158,32 +89,13 @@ Section MultiThread.
       (Closed.final_state ClosedS) ls i->
       final_state s i.
 
-  (** * Definitions about the primitive yield *)
-
-  Definition yield_id := 1001%positive.
-  Definition yield_sig := mksignature nil Tvoid cc_default.
-
-  Inductive query_is_yield : query li_c -> Prop :=
+  
+  (** * Operations about *)
+  Inductive query_is_yield : query li_asm -> Prop :=
   |yield_intro : forall b m,
     Genv.find_symbol initial_se yield_id = Some b ->
     query_is_yield (cq (Vptr b Ptrofs.zero) yield_sig nil m).
 
-  (** * Definitions about the primitive pthread_create *)
-
-  Definition pthread_create_id := 1002%positive.
-  
-
-  (* TODO: not quite sure to use Tlong or Tany64 here, we used Tlong for function pointer in the Client-Server example *)
-  (** int pthread_create (void * (*start_routine) (void*), void* arg) *)
-  Definition pthread_create_sig := mksignature (Tlong :: Tlong :: nil) Tint cc_default.
-
-  
-  (** Problem here: the type of start_routine here may not be accecpted by [initial_state] in Clight semantics. *)
-  (** Maybe we have to do sth more to support such void* (*f) (void*) prototype, maybe not using cc_default *)
-  Definition start_routine_sig := mksignature (Tlong :: nil) Tlong cc_default.
-
-
-  (* turns a call to pthread_create into a call to the start_routine, the initial memory is updated in 2nd query *)
   Inductive query_is_pthread_create : query li_c -> query li_c -> Prop :=
   |pthread_create_intro :
     forall m arglist b_ptc b_start b_arg ofs m'
@@ -194,6 +106,16 @@ Section MultiThread.
         (cq (Vptr b_ptc Ptrofs.zero) pthread_create_sig arglist m)
         (cq (Vptr b_start Ptrofs.zero) start_routine_sig ((Vptr b_arg ofs)::nil) m').
 
+  Inductive query_is_pthread_create : query li_c -> query li_c -> Prop :=
+  |pthread_create_intro :
+    forall m arglist b_ptc b_start b_arg ofs m'
+      (FINDPTC: Genv.find_symbol initial_se pthread_create_id = Some b_ptc)
+      (ARGLIST: arglist = (Vptr b_start Ptrofs.zero) :: (Vptr b_arg ofs) :: nil)
+      (MEM_CREATE: Mem.thread_create m = m'),
+      query_is_pthread_create
+        (cq (Vptr b_ptc Ptrofs.zero) pthread_create_sig arglist m)
+        (cq (Vptr b_start Ptrofs.zero) start_routine_sig ((Vptr b_arg ofs)::nil) m').
+  
   
   Inductive step : genvtype -> state -> trace -> state -> Prop :=
   |step_local : forall ge ls1 t ls2 s s',
@@ -236,4 +158,3 @@ Section MultiThread.
       step ge s E0 s'.
   
 End MultiThread.   
-  
