concur/AsmMulti.v
@@ -1,0 +1,193 @@
+Require Import Relations.
+Require Import Wellfounded.
+Require Import Coqlib.
+Require Import Errors.
+Require Import Events.
+Require Import Globalenvs.
+Require Import LanguageInterface.
+Require Import Integers.
+Require Import Smallstep.
+Require Import SmallstepClosed.
+Require Import Values Maps Memory AST.
+
+Require Import Asm SmallstepMulti.
+
+Section MultiThread.
+  
+  Context {OpenS: Smallstep.semantics li_asm li_asm}.
+
+  Definition local_state := Smallstep.state OpenS.
+
+  Definition thread_state : Type := local_state + regset.
+
+  Variable initial_query : query li_asm.
+  Variable final_reply : int -> reply li_asm -> Prop.
+
+  Variable initial_se : Genv.symtbl.
+
+  Definition OpenLTS := activate OpenS initial_se.
+  Definition ClosedS := Closed.close_semantics initial_query final_reply OpenS initial_se.
+
+  Record state : Type := mk_gstate_asm
+      {
+        threads : NatMap.t (option thread_state);
+        cur_tid : nat;
+        next_tid : nat;
+      }.
+
+  Definition empty_threads : NatMap.t (option thread_state) := NatMap.init None.
+  
+  Definition update_threads (s: state) (t: NatMap.t (option thread_state)) :=
+    mk_gstate_asm t (cur_tid s) (next_tid s) .
+
+  Definition update_thread (s: state) (tid : nat) (ls: thread_state) :=
+    mk_gstate_asm (NatMap.set tid (Some ls) (threads s)) (cur_tid s) (next_tid s).
+
+  Definition update_cur_thread (s: state) (ls : thread_state) := update_thread s (cur_tid s) ls.
+  
+  Definition get_thread (s: state) (tid: nat) :=
+    NatMap.get tid (threads s).
+
+  Definition get_cur_thread (s: state) := get_thread s (cur_tid s).
+  
+  Definition update_cur_tid (s: state) (tid : nat) :=
+    mk_gstate_asm (threads s) tid (next_tid s).
+
+  Definition update_next_tid (s: state) (tid: nat) :=
+    mk_gstate_asm (threads s) (cur_tid s) tid.
+  
+  Variable yield_strategy : state -> nat.
+  Axiom yield_strategy_range : forall s, (1 < yield_strategy s < (next_tid s))%nat.
+
+  Definition yield_state (s: state) (ls: thread_state): state :=
+    let tid' := yield_strategy s in
+    let s' := update_cur_tid s tid' in
+    update_thread s' tid' ls.
+
+  (* We add a new thread with its initial query without memory,
+      we also update the running memory by adding a new list of positives *)
+  Definition pthread_create_state (s: state) (regs: regset) (ls' : thread_state): state :=
+    let ntid := (next_tid s) in let ctid := (cur_tid s) in
+    let s' := update_next_tid s (S ntid) in
+    let s'' := update_thread s' ntid (inr regs) in
+    update_thread s'' ctid ls'.
+    
+  Definition genvtype := Smallstep.genvtype OpenLTS.
+  
+  Inductive initial_state : state -> Prop :=
+  |initial_state_intro : forall ls s,
+      cur_tid s = 1%nat -> next_tid s = 2%nat ->
+      get_cur_thread s = Some (inl ls) ->
+      (Closed.initial_state ClosedS) ls ->
+      initial_state s.
+
+  (** Final state of Concurrent semantics *)
+  Inductive final_state : state -> int -> Prop :=  
+  |final_state_intro : forall ls i s,
+      cur_tid s = 1%nat ->
+      get_cur_thread s = Some (inl ls) ->
+      (Closed.final_state ClosedS) ls i->
+      final_state s i.
+
+  
+  (** * Operations about dealing with queries *)
+
+
+  (* We should not define it like this, it's tautoloty
+  Inductive query_is_yield_asm : query li_asm -> Prop :=
+  |yield_intro : forall rs m q_c,
+      query_is_yield qc ->
+      cc_c_asm_mq (caw yield_sig rs m) qc (rs,m) ->
+      query_is_yield (rs, m). *)
+
+  (* Print yield_sig.
+     yield_sig = {| sig_args := nil; sig_res := Tvoid; sig_cc := cc_default |}
+     : signature
+   *)
+
+  Inductive query_is_yield_asm : query li_asm -> Prop :=
+  |yield_intro_asm : forall rs m b,
+      Genv.find_symbol initial_se yield_id = Some b ->
+      rs # PC = Vptr b Ptrofs.zero ->
+      query_is_yield_asm (rs, m).
+
+  (*
+  pthread_create_sig = 
+{| sig_args := Tlong :: Tlong :: nil; sig_res := Tint; sig_cc := cc_default |}
+     : signature
+ *)
+
+  Require Import Conventions1.
+  
+  Axiom not_win : Archi.win64 = false.
+  
+  (* the ptr to start_routine is in RDI, the pointer to its argument is in RSI *)
+  Theorem pthread_create_locs :
+    loc_arguments pthread_create_sig = One (Locations.R Machregs.DI) :: One (Locations.R Machregs.SI) :: nil.
+  Proof.
+    simpl. unfold pthread_create_sig. unfold loc_arguments.
+    replace Archi.ptr64 with true by reflexivity.
+    rewrite not_win. simpl. reflexivity.
+  Qed.
+
+  (* the pointer to the arg of start_routine should be placed in RDI for new thread regs *)
+  Theorem start_routine_loc :
+    loc_arguments start_routine_sig = One (Locations.R Machregs.DI) :: nil.
+  Proof.
+    simpl.  simpl. unfold pthread_create_sig. unfold loc_arguments.
+    replace Archi.ptr64 with true by reflexivity.
+    rewrite not_win. simpl. reflexivity.
+  Qed.
+  
+  Inductive query_is_pthread_create_asm : query li_asm -> query li_asm -> Prop :=
+  |pthread_create_intro :
+    forall m b_ptc b_start b_arg ofs m' rs rs'
+      (FINDPTC: Genv.find_symbol initial_se pthread_create_id = Some b_ptc)
+      (RS_PC: rs # PC = Vptr b_ptc Ptrofs.zero)
+      (RS_RDI : rs # RDI = Vptr b_start Ptrofs.zero)
+      (RS_RSI : rs # RSI = Vptr b_arg ofs)
+      (RS'_PC : rs' # PC = Vptr b_start Ptrofs.zero)
+      (rs'_RDI : rs' # RDI = Vptr b_arg ofs)
+      (** We may need more requirements of rs' here *)
+      (MEM_CREATE: Mem.thread_create m = m'),
+      query_is_pthread_create_asm (rs,m) (rs', m').
+  
+  Inductive step : genvtype -> state -> trace -> state -> Prop :=
+  |step_local : forall ge ls1 t ls2 s s',
+      get_cur_thread s = Some (inl ls1) ->
+      Smallstep.step OpenLTS ge ls1 t ls2 ->
+      update_thread s (cur_tid s) (inl ls2) = s' ->
+      step ge s t s'
+  |step_thread_create : forall ge s s' q_ptc rs_str gmem ls ls',
+      get_cur_thread s = Some (inl ls) -> (* get the current local state *)
+      Smallstep.at_external OpenLTS ls q_ptc -> (* get the query to pthread_create *)
+      query_is_pthread_create_asm q_ptc (rs_str, gmem) -> (* get the query to start_routine *)
+      Smallstep.after_external OpenLTS ls (fst q_ptc, gmem) ls' ->
+      (* the current thread completes the primitive, regsets are unchanged *)
+      pthread_create_state s rs_str (inl ls') = s' ->
+      step ge s E0 s'.
+  (** yield to a thread which is waiting for the reply of its own [yield()] *)
+  |step_thread_yield_to_yield : forall ge s s' tid' q gmem' p ls ls1 ls1',
+      get_cur_thread s = Some (inl ls) ->
+      Smallstep.at_external OpenLTS ls q ->
+      query_is_yield q ->
+      yield_strategy s = tid' ->
+      (*the proof p may be a problem, provided from the invariant between state and the support in gmem *)
+      Mem.yield (cq_mem q) tid' p = gmem' ->
+      get_thread s (tid') = Some (inl ls1) -> (* the target thread is waiting for reply *)
+      Smallstep.after_external OpenLTS ls1 (cr Vundef gmem') ls1' ->
+      yield_state s (inl ls1') = s' ->
+      step ge s E0 s'
+  (** yield to a thread which has not been initialized from a query *)
+  |step_thread_yield_to_initial : forall ge s s' tid' q gmem' p ls cqv ls1',
+      get_cur_thread s = Some (inl ls) ->
+      Smallstep.at_external OpenLTS ls q ->
+      query_is_yield q ->
+      yield_strategy s = tid' ->
+      Mem.yield (cq_mem q) tid' p = gmem' ->
+      get_thread s (tid') = Some (inr cqv) -> (* the target thread is waiting for reply *)
+      Smallstep.initial_state OpenLTS (get_query cqv gmem') ls1' ->
+      yield_state s (inl ls1') = s' ->
+      step ge s E0 s'.
+  
+End MultiThread.   
