concur/SmallstepMulti.v
@@ -1,0 +1,239 @@
+Require Import Relations.
+Require Import Wellfounded.
+Require Import Coqlib.
+Require Import Errors.
+Require Import Events.
+Require Import Globalenvs.
+Require Import LanguageInterface.
+Require Import Integers.
+Require Import Smallstep.
+Require Import SmallstepClosed.
+Require Import Values Maps Memory AST.
+
+Module NatIndexed.
+    Definition t := nat.
+
+    Definition index (n : nat) : positive :=
+      match n with
+      |O => 1%positive
+      |_ => 1 + Pos.of_nat n
+      end.
+
+    Definition index_rev (p:positive) : nat :=
+      match p with
+      |xH => O
+      |_ => Pos.to_nat p -1
+    end.
+
+    Lemma t_positive_t : forall (n:nat), index_rev (index n) = n.
+    Proof.
+      intros.
+      destruct (index n) eqn:Hn; unfold index_rev; destruct n; unfold index in *; lia.
+    Qed.
+
+    Lemma positive_t_positive : forall (p:positive), index(index_rev p) = p.
+    Proof.
+      intros. destruct (index_rev p) eqn:Hp; unfold index; destruct p; unfold index_rev in *; lia.
+    Qed.
+
+    Lemma index_inj : forall (x y : nat), index x = index y -> x = y.
+    Proof.
+      destruct x; destruct y; unfold index in *; lia.
+    Qed.
+    
+    Definition eq := Nat.eq_dec.
+End NatIndexed.
+
+Module NatMap := IRMap(NatIndexed).
+
+(** Unchecked concern: Do we need to define new events for [yield] and [pthread_create] ? Can we keep the internal events?
+    Now this two points are implemented differernt with CASCompCert *)
+Section MultiThread.
+
+  Context {OpenS : semantics li_c li_c}.
+
+  Definition local_state := state OpenS.
+
+  Record cq_vals : Type := cqv {cqv_vf : val; cqv_sg : signature; cqv_args : list val}.
+
+  Definition get_query (cqv : cq_vals) (m: mem) :=
+    cq (cqv_vf cqv) (cqv_sg cqv) (cqv_args cqv) m.
+
+  Definition get_cqv (q: c_query) :=
+    cqv (cq_vf q) (cq_sg q) (cq_args q).
+  
+  Definition thread_state :Type := local_state + cq_vals.
+  
+  (* Maybe should be somehow added into open semantics *)
+  Variable initial_query : query li_c.
+  Variable final_reply : int -> reply li_c -> Prop.
+
+  (* should be derived from skel of OpenS
+     and allocate blocks for pthread primitives *)
+  Variable initial_se : Genv.symtbl.
+  
+  Definition OpenLTS := activate OpenS initial_se.
+  Definition ClosedS := Closed.close_semantics initial_query final_reply OpenS initial_se.
+
+  (* We need an interface to get and set global memory from local_state *)
+  (* Not sure if this is proper, maybe need some lemmas about these operations *)
+
+  (*Variable get_gmem : local_state -> mem.
+  Variable set_gmem : mem -> local_state -> local_state. *)
+  
+  (** * Definition and operations of global state *)
+
+    Record state : Type := mk_gstate
+    {
+      threads: NatMap.t (option thread_state);
+      cur_tid : nat;
+      next_tid : nat;
+      (* atom_bit : bool; *)
+
+      (* tid_gmem : exists ls, NatMap.get cur_tid threads = Some ls /\
+                         tid_mem (get_gmem ls) = cur_tid /\
+                         length (stacks_mem (get_gmem ls)) = next_tid; *)
+    }.
+
+  Definition empty_threads : NatMap.t (option thread_state) := NatMap.init None.
+  
+  Definition update_threads (s: state) (t: NatMap.t (option thread_state)) :=
+    mk_gstate t (cur_tid s) (next_tid s) .
+
+  Definition update_thread (s: state) (tid : nat) (ls: thread_state) :=
+    mk_gstate (NatMap.set tid (Some ls) (threads s)) (cur_tid s) (next_tid s).
+
+  Definition update_cur_thread (s: state) (ls : thread_state) := update_thread s (cur_tid s) ls.
+  
+  Definition get_thread (s: state) (tid: nat) :=
+    NatMap.get tid (threads s).
+
+  Definition get_cur_thread (s: state) := get_thread s (cur_tid s).
+  
+  Definition update_cur_tid (s: state) (tid : nat) :=
+    mk_gstate (threads s) tid (next_tid s).
+
+  Definition update_next_tid (s: state) (tid: nat) :=
+    mk_gstate (threads s) (cur_tid s) tid.
+  
+  Variable yield_strategy : state -> nat.
+  Axiom yield_strategy_range : forall s, (1 < yield_strategy s < (next_tid s))%nat.
+  (*some other properties may be added here, such as only point to active threads *)
+
+  (* We transfer to thread tid' and update
+     its local_state with an updated memory *)
+
+  Definition yield_state (s: state) (ls: thread_state): state :=
+    let tid' := yield_strategy s in
+    let s' := update_cur_tid s tid' in
+    update_thread s' tid' ls.
+
+  (* We add a new thread with its initial query without memory,
+      we also update the running memory by adding a new list of positives *)
+  Definition pthread_create_state (s: state) (cqv : cq_vals) (ls' : thread_state): state :=
+    let ntid := (next_tid s) in let ctid := (cur_tid s) in
+    let s' := update_next_tid s (S ntid) in
+    let s'' := update_thread s' ntid (inr cqv) in
+    update_thread s'' ctid ls'.
+    
+  Definition genvtype := Smallstep.genvtype OpenLTS.
+  
+  (** Initial state of Concurrent semantics *)
+
+  (* We need a "query" to the main function of the semantics *)
+  (* Including the initial global memory *)
+
+  Inductive initial_state : state -> Prop :=
+  |initial_state_intro : forall ls s,
+      cur_tid s = 1%nat -> next_tid s = 2%nat ->
+      get_cur_thread s = Some (inl ls) ->
+      (Closed.initial_state ClosedS) ls ->
+      initial_state s.
+
+  (** Final state of Concurrent semantics *)
+  Inductive final_state : state -> int -> Prop :=  
+  |final_state_intro : forall ls i s,
+      cur_tid s = 1%nat ->
+      get_cur_thread s = Some (inl ls) ->
+      (Closed.final_state ClosedS) ls i->
+      final_state s i.
+
+  (** * Definitions about the primitive yield *)
+
+  Definition yield_id := 1001%positive.
+  Definition yield_sig := mksignature nil Tvoid cc_default.
+
+  Inductive query_is_yield : query li_c -> Prop :=
+  |yield_intro : forall b m,
+    Genv.find_symbol initial_se yield_id = Some b ->
+    query_is_yield (cq (Vptr b Ptrofs.zero) yield_sig nil m).
+
+  (** * Definitions about the primitive pthread_create *)
+
+  Definition pthread_create_id := 1002%positive.
+  
+
+  (* TODO: not quite sure to use Tlong or Tany64 here, we used Tlong for function pointer in the Client-Server example *)
+  (** int pthread_create (void * (*start_routine) (void*), void* arg) *)
+  Definition pthread_create_sig := mksignature (Tlong :: Tlong :: nil) Tint cc_default.
+
+  
+  (** Problem here: the type of start_routine here may not be accecpted by [initial_state] in Clight semantics. *)
+  (** Maybe we have to do sth more to support such void* (*f) (void*) prototype, maybe not using cc_default *)
+  Definition start_routine_sig := mksignature (Tlong :: nil) Tlong cc_default.
+
+
+  (* turns a call to pthread_create into a call to the start_routine, the initial memory is updated in 2nd query *)
+  Inductive query_is_pthread_create : query li_c -> query li_c -> Prop :=
+  |pthread_create_intro :
+    forall m arglist b_ptc b_start b_arg ofs m'
+      (FINDPTC: Genv.find_symbol initial_se pthread_create_id = Some b_ptc)
+      (ARGLIST: arglist = (Vptr b_start Ptrofs.zero) :: (Vptr b_arg ofs) :: nil)
+      (MEM_CREATE: Mem.thread_create m = m'),
+      query_is_pthread_create
+        (cq (Vptr b_ptc Ptrofs.zero) pthread_create_sig arglist m)
+        (cq (Vptr b_start Ptrofs.zero) start_routine_sig ((Vptr b_arg ofs)::nil) m').
+
+  
+  Inductive step : genvtype -> state -> trace -> state -> Prop :=
+  |step_local : forall ge ls1 t ls2 s s',
+      get_cur_thread s = Some (inl ls1) ->
+      Smallstep.step OpenLTS ge ls1 t ls2 ->
+      update_thread s (cur_tid s) (inl ls2) = s' ->
+      step ge s t s'
+  |step_thread_create : forall ge s s' q_ptc q_str gmem ls ls' cqv,
+      get_cur_thread s = Some (inl ls) -> (* get the current local state *)
+      Smallstep.at_external OpenLTS ls q_ptc -> (* get the query to pthread_create *)
+      query_is_pthread_create q_ptc q_str -> (* get the query to start_routine *)
+      (* The global memory is already updated from q_ptc to q_str *)
+      cq_mem q_str = gmem -> (* the updated memory, only difference is the #threads *)
+      get_cqv q_str = cqv -> (*the initial query without memory, is stored as initial state in new thread *)
+      Smallstep.after_external OpenLTS ls (cr (Vint Int.one) gmem) ls' -> (* the current thread completes the primitive*)
+      pthread_create_state s cqv (inl ls') = s' ->
+      step ge s E0 s'
+  (** yield to a thread which is waiting for the reply of its own [yield()] *)
+  |step_thread_yield_to_yield : forall ge s s' tid' q gmem' p ls ls1 ls1',
+      get_cur_thread s = Some (inl ls) ->
+      Smallstep.at_external OpenLTS ls q ->
+      query_is_yield q ->
+      yield_strategy s = tid' ->
+      (*the proof p may be a problem, provided from the invariant between state and the support in gmem *)
+      Mem.yield (cq_mem q) tid' p = gmem' ->
+      get_thread s (tid') = Some (inl ls1) -> (* the target thread is waiting for reply *)
+      Smallstep.after_external OpenLTS ls1 (cr Vundef gmem') ls1' ->
+      yield_state s (inl ls1') = s' ->
+      step ge s E0 s'
+  (** yield to a thread which has not been initialized from a query *)
+  |step_thread_yield_to_initial : forall ge s s' tid' q gmem' p ls cqv ls1',
+      get_cur_thread s = Some (inl ls) ->
+      Smallstep.at_external OpenLTS ls q ->
+      query_is_yield q ->
+      yield_strategy s = tid' ->
+      Mem.yield (cq_mem q) tid' p = gmem' ->
+      get_thread s (tid') = Some (inr cqv) -> (* the target thread is waiting for reply *)
+      Smallstep.initial_state OpenLTS (get_query cqv gmem') ls1' ->
+      yield_state s (inl ls1') = s' ->
+      step ge s E0 s'.
+  
+End MultiThread.   
+
